chore: renaming

CollapsingTowers/TwoLevelRec/LogicalEquiv/LogicalRelation.lean
@@ -2,7 +2,7 @@ import CollapsingTowers.TwoLevelRec.SyntacticTyping.Defs
 
 mutual
 @[simp]
-def logic_rel_value : ℕ → Expr → Expr → Ty → Prop
+def log_rel_value : ℕ → Expr → Expr → Ty → Prop
   --
   --
   -- 𝓥⟦ℕ⟧ₖ ≜ {(n, n) | n ∈ ℕ}
@@ -19,8 +19,8 @@ def logic_rel_value : ℕ → Expr → Expr → Ty → Prop
     typing [] 𝟙 (.lam e₁) (.arrow τ𝕒 τ𝕓 ∅) ∅ ∧
     ∀ j, j ≤ k →
       ∀ v₀ v₁,
-        logic_rel_value j v₀ v₁ τ𝕒 →
-        logic_rel_expr j (.app₁ (.lam e₀) v₀) (.app₁ (.lam e₁) v₁) τ𝕓
+        log_rel_value j v₀ v₁ τ𝕒 →
+        log_rel_expr j (.app₁ (.lam e₀) v₀) (.app₁ (.lam e₁) v₁) τ𝕓
   | _, _, _, _ => false
 
 termination_by k _ _ τ => (τ, k)
@@ -28,45 +28,45 @@ decreasing_by all_goals apply Prod.Lex.left; simp; omega
 
 -- 𝓔⟦τ⟧ₖ ≜ {(e₀, e₁) | ∀ j < k, v₀. e₀ ⇾ⱼ v₀ → ∃ v₁, e₁ ⇾* v₁ ∧ (v₀, v₁) ∈ 𝓥⟦τ⟧ₖ₋ⱼ}
 @[simp]
-def logic_rel_expr (k : ℕ) (e₀ : Expr) (e₁ : Expr) (τ : Ty) : Prop :=
+def log_rel_expr (k : ℕ) (e₀ : Expr) (e₁ : Expr) (τ : Ty) : Prop :=
     ∀ j, j < k →
       ∀ v₀, value v₀ → (e₀ ⇾ ⟦j⟧ v₀) →
-      ∃ v₁, (e₁ ⇾* v₁) ∧ logic_rel_value (k - j) v₀ v₁ τ
+      ∃ v₁, (e₁ ⇾* v₁) ∧ log_rel_value (k - j) v₀ v₁ τ
 
 termination_by (τ, k + 1)
 decreasing_by apply Prod.Lex.right; omega
 end
 
-inductive logic_rel_env : ℕ → Subst → Subst → TEnv → Prop where
-  | nil : ∀ k, logic_rel_env k [] [] []
+inductive log_rel_env : ℕ → Subst → Subst → TEnv → Prop where
+  | nil : ∀ k, log_rel_env k [] [] []
   | cons :
     ∀ k v₀ γ₀ v₁ γ₁ τ Γ,
-      logic_rel_value k v₀ v₁ τ →
-      logic_rel_env k γ₀ γ₁ Γ →
-      logic_rel_env k (v₀ :: γ₀) (v₁ :: γ₁) ((τ, 𝟙) :: Γ)
+      log_rel_value k v₀ v₁ τ →
+      log_rel_env k γ₀ γ₁ Γ →
+      log_rel_env k (v₀ :: γ₀) (v₁ :: γ₁) ((τ, 𝟙) :: Γ)
 
 -- Γ ⊧ e₀ ≤𝑙𝑜𝑔 e₁ : τ ≜
 --   Γ ⊢ λx.e₀ : τ𝕒 → τ𝕓 ∧
 --   Γ ⊢ λx.e₀ : τ𝕒 → τ𝕓 ∧
 --   ∀ k ≥ 0, (γ₀, γ₁) ∈ 𝓖⟦Γ⟧ₖ. (γ₀(e₀), γ₁(e₁)) ∈ 𝓔⟦τ⟧ₖ
 @[simp]
-def logic_rel_typing (Γ : TEnv) (e₀ : Expr) (e₁ : Expr) (τ : Ty) : Prop :=
+def log_rel_typing (Γ : TEnv) (e₀ : Expr) (e₁ : Expr) (τ : Ty) : Prop :=
   typing Γ 𝟙 e₀ τ ∅ ∧
   typing Γ 𝟙 e₁ τ ∅ ∧
   ∀ k γ₀ γ₁,
-    logic_rel_env k γ₀ γ₁ Γ →
-    logic_rel_expr k (multi_subst γ₀ e₀) (multi_subst γ₁ e₁) τ
+    log_rel_env k γ₀ γ₁ Γ →
+    log_rel_expr k (multi_subst γ₀ e₀) (multi_subst γ₁ e₁) τ
 
 -- Γ ⊧ e₀ ≈𝑙𝑜𝑔 e₁ : τ ≜ Γ ⊧ e₀ ≤𝑙𝑜𝑔 e₁ : τ ∧ Γ ⊧ e₁ ≤𝑙𝑜𝑔 e₀ : τ
 @[simp]
-def logic_equiv (Γ : TEnv) (e₀ : Expr) (e₁ : Expr) (τ : Ty) : Prop :=
-  logic_rel_typing Γ e₀ e₁ τ ∧ logic_rel_typing Γ e₁ e₀ τ
+def log_equiv (Γ : TEnv) (e₀ : Expr) (e₁ : Expr) (τ : Ty) : Prop :=
+  log_rel_typing Γ e₀ e₁ τ ∧ log_rel_typing Γ e₁ e₀ τ
 
-lemma logic_rel_value.antimono :
+lemma log_rel_value.antimono :
   ∀ k₀ k₁ v₀ v₁ τ,
-    logic_rel_value k₀ v₀ v₁ τ →
+    log_rel_value k₀ v₀ v₁ τ →
     k₁ ≤ k₀ →
-    logic_rel_value k₁ v₀ v₁ τ :=
+    log_rel_value k₁ v₀ v₁ τ :=
   by
   intros k₀ k₁ v₀ v₁ τ Hsem_value HLe
   cases τ
@@ -81,48 +81,48 @@ lemma logic_rel_value.antimono :
     cases φ
     case reify => simp at Hsem_value
     case pure =>
-      simp only [logic_rel_value] at Hsem_value
+      simp only [log_rel_value] at Hsem_value
       have ⟨Hτ₀, Hτ₁, Hsem_value_lam⟩ := Hsem_value
-      simp only [logic_rel_value]
+      simp only [log_rel_value]
       constructor; apply Hτ₀
       constructor; apply Hτ₁
       intros j HLe; apply Hsem_value_lam; omega
   case fragment => simp at Hsem_value
   case rep => simp at Hsem_value
 
-lemma logic_rel_expr.antimono :
+lemma log_rel_expr.antimono :
   ∀ k₀ k₁ e₀ e₁ τ,
-    logic_rel_expr k₀ e₀ e₁ τ →
+    log_rel_expr k₀ e₀ e₁ τ →
     k₁ ≤ k₀ →
-    logic_rel_expr k₁ e₀ e₁ τ :=
+    log_rel_expr k₁ e₀ e₁ τ :=
   by
   intros k₀ k₁ e₀ e₁ τ Hsem_expr HLe
-  simp only [logic_rel_expr]
-  simp only [logic_rel_expr] at Hsem_expr
+  simp only [log_rel_expr]
+  simp only [log_rel_expr] at Hsem_expr
   intros j Hindex v₀ Hvalue₀ Hstep₀
   have ⟨v₁, Hstep₁, Hsem_value⟩ := Hsem_expr j (by omega) v₀ Hvalue₀ Hstep₀
   exists v₁
   constructor; apply Hstep₁
-  apply logic_rel_value.antimono
+  apply log_rel_value.antimono
   apply Hsem_value; omega
 
-lemma logic_rel_env.antimono :
+lemma log_rel_env.antimono :
   ∀ k₀ k₁ γ₀ γ₁ Γ,
-    logic_rel_env k₀ γ₀ γ₁ Γ →
+    log_rel_env k₀ γ₀ γ₁ Γ →
     k₁ ≤ k₀ →
-    logic_rel_env k₁ γ₀ γ₁ Γ :=
+    log_rel_env k₁ γ₀ γ₁ Γ :=
   by
   intros k₀ k₁ γ₀ γ₁ Γ HsemΓ HLe
   induction HsemΓ
-  case nil => apply logic_rel_env.nil
+  case nil => apply log_rel_env.nil
   case cons Hsem_value _ IH =>
-    apply logic_rel_env.cons
-    apply logic_rel_value.antimono; apply Hsem_value; apply HLe
+    apply log_rel_env.cons
+    apply log_rel_value.antimono; apply Hsem_value; apply HLe
     apply IH
 
-lemma logic_rel_value.syntactic.value :
+lemma log_rel_value.syntactic.value :
   ∀ k v₀ v₁ τ,
-    logic_rel_value k v₀ v₁ τ →
+    log_rel_value k v₀ v₁ τ →
     value v₀ ∧ value v₁ :=
   by
   intros k v₀ v₁ τ Hsem_value
@@ -140,9 +140,9 @@ lemma logic_rel_value.syntactic.value :
     apply value.lam; apply typing.regular; apply Hτ₁
   all_goals simp at Hsem_value
 
-lemma logic_rel_value.syntactic.typing :
+lemma log_rel_value.syntactic.typing :
   ∀ k v₀ v₁ τ,
-    logic_rel_value k v₀ v₁ τ →
+    log_rel_value k v₀ v₁ τ →
     typing [] 𝟙 v₀ τ ∅ ∧ typing [] 𝟙 v₁ τ ∅ :=
   by
   intros k v₀ v₁ τ Hsem_value
@@ -156,20 +156,20 @@ lemma logic_rel_value.syntactic.typing :
     constructor; apply Hτ₀; apply Hτ₁
   all_goals simp at Hsem_value
 
-lemma logic_rel_value.apply :
+lemma log_rel_value.apply :
   ∀ k f₀ arg₀ f₁ arg₁ τ𝕒 τ𝕓,
-    logic_rel_value k f₀ f₁ (.arrow τ𝕒 τ𝕓 ∅) →
-    logic_rel_value k arg₀ arg₁ τ𝕒 →
-    logic_rel_expr k (.app₁ f₀ arg₀) (.app₁ f₁ arg₁) τ𝕓 :=
+    log_rel_value k f₀ f₁ (.arrow τ𝕒 τ𝕓 ∅) →
+    log_rel_value k arg₀ arg₁ τ𝕒 →
+    log_rel_expr k (.app₁ f₀ arg₀) (.app₁ f₁ arg₁) τ𝕓 :=
   by
   intros k f₀ arg₀ f₁ arg₁ τ𝕒 τ𝕓 Hsem_value_fun Hsem_value_arg
-  cases f₀ <;> cases f₁ <;> simp only [logic_rel_value] at Hsem_value_fun <;> try contradiction
+  cases f₀ <;> cases f₁ <;> simp only [log_rel_value] at Hsem_value_fun <;> try contradiction
   have ⟨_, _, Hsem_value_fun⟩ := Hsem_value_fun
   apply Hsem_value_fun; rfl; apply Hsem_value_arg
 
-lemma logic_rel_env.length :
+lemma log_rel_env.length :
   ∀ k γ₀ γ₁ Γ,
-    logic_rel_env k γ₀ γ₁ Γ →
+    log_rel_env k γ₀ γ₁ Γ →
     γ₀.length = Γ.length ∧
     γ₁.length = Γ.length :=
   by
@@ -181,18 +181,18 @@ lemma logic_rel_env.length :
     . simp; apply IH.left
     . simp; apply IH.right
 
-lemma logic_rel_env.binds_logic_rel_value :
+lemma log_rel_env.binds_log_rel_value :
   ∀ k γ₀ γ₁ Γ x τ,
-    logic_rel_env k γ₀ γ₁ Γ →
+    log_rel_env k γ₀ γ₁ Γ →
     binds x (τ, 𝟙) Γ →
-    logic_rel_value k (multi_subst γ₀ (.fvar x)) (multi_subst γ₁ (.fvar x)) τ :=
+    log_rel_value k (multi_subst γ₀ (.fvar x)) (multi_subst γ₁ (.fvar x)) τ :=
   by
   intros k γ₀ γ₁ Γ x τ HsemΓ Hbinds
   induction HsemΓ
   case nil => nomatch Hbinds
   case cons v₀ γ₀ v₁ γ₁ τ Γ Hsem_value HsemΓ IH =>
-    have ⟨Hτ₀, Hτ₁⟩ := logic_rel_value.syntactic.typing _ _ _ _ Hsem_value
-    have ⟨HEq₀, HEq₁⟩ := logic_rel_env.length _ _ _ _ HsemΓ
+    have ⟨Hτ₀, Hτ₁⟩ := log_rel_value.syntactic.typing _ _ _ _ Hsem_value
+    have ⟨HEq₀, HEq₁⟩ := log_rel_env.length _ _ _ _ HsemΓ
     simp [HEq₀, HEq₁]
     by_cases HEqx : Γ.length = x
     . simp [if_pos HEqx]
@@ -205,16 +205,16 @@ lemma logic_rel_env.binds_logic_rel_value :
       simp [if_neg HEqx] at Hbinds
       apply IH; apply Hbinds
 
-lemma logic_rel_env.multi_wf :
+lemma log_rel_env.multi_wf :
   ∀ k γ₀ γ₁ Γ,
-    logic_rel_env k γ₀ γ₁ Γ →
+    log_rel_env k γ₀ γ₁ Γ →
     multi_wf γ₀ ∧ multi_wf γ₁ :=
   by
   intros k γ₀ γ₁ Γ HsemΓ
   induction HsemΓ
   case nil => repeat constructor
   case cons Hsem_value _ IH =>
-    have ⟨Hτ₀, Hτ₁⟩ := logic_rel_value.syntactic.typing _ _ _ _ Hsem_value
+    have ⟨Hτ₀, Hτ₁⟩ := log_rel_value.syntactic.typing _ _ _ _ Hsem_value
     constructor
     . constructor
       apply typing.wf []; apply Hτ₀
@@ -223,11 +223,11 @@ lemma logic_rel_env.multi_wf :
       apply typing.wf []; apply Hτ₁
       apply IH.right
 
-lemma logic_rel_env.subst.typing :
+lemma log_rel_env.subst.typing :
   ∀ k γ₀ γ₁ e₀ e₁ Γ τ,
     typing Γ 𝟙 e₀ τ ∅ →
     typing Γ 𝟙 e₁ τ ∅ →
-    logic_rel_env k γ₀ γ₁ Γ →
+    log_rel_env k γ₀ γ₁ Γ →
     typing [] 𝟙 (multi_subst γ₀ e₀) τ ∅ ∧
     typing [] 𝟙 (multi_subst γ₁ e₁) τ ∅ :=
   by
@@ -235,8 +235,8 @@ lemma logic_rel_env.subst.typing :
   induction HsemΓ generalizing e₀ e₁
   case nil => constructor; apply Hτ₀; apply Hτ₁
   case cons Γ Hsem_value HsemΓ IH =>
-    have ⟨HEq₀, HEq₁⟩ := logic_rel_env.length _ _ _ _ HsemΓ
-    have ⟨Hτv₀, Hτv₁⟩ := logic_rel_value.syntactic.typing _ _ _ _ Hsem_value
+    have ⟨HEq₀, HEq₁⟩ := log_rel_env.length _ _ _ _ HsemΓ
+    have ⟨Hτv₀, Hτv₁⟩ := log_rel_value.syntactic.typing _ _ _ _ Hsem_value
     apply IH
     . rw [HEq₀]; apply preservation.subst; rw [← List.append_nil Γ]
       apply typing.weakening; apply Hτv₀; apply Hτ₀
