CollapsingTowers/TwoLevelRec/Defs.lean
@@ -4,4 +4,4 @@ import CollapsingTowers.TwoLevelRec.OperationalSemantics.Defs
 import CollapsingTowers.TwoLevelRec.SyntacticTyping.Defs
 import CollapsingTowers.TwoLevelRec.Erasure.Defs
 import CollapsingTowers.TwoLevelRec.CtxEquiv.Defs
-import CollapsingTowers.TwoLevelRec.LogicEquiv.Defs
+import CollapsingTowers.TwoLevelRec.LogicalEquiv.Defs
