CollapsingTowers/TwoLevelRec/LogicalEquiv/Defs.lean
@@ -1,0 +1,4 @@
+import CollapsingTowers.TwoLevelRec.LogicalEquiv.LogicalRelation
+import CollapsingTowers.TwoLevelRec.LogicalEquiv.Compatibility
+import CollapsingTowers.TwoLevelRec.LogicalEquiv.Fundamental
+import CollapsingTowers.TwoLevelRec.LogicalEquiv.Soundness
